Updates.

LC/NV/UTLC/Sub/IsSub.lean
@@ -13,10 +13,75 @@ set_option autoImplicit false
 open Term_
 
 
+inductive is_sub_v0 : Term_ → Symbol_ → Term_ → Term_ → Prop
+
+-- if x = y then y [ x := N ] = N
+| var_same
+  (y : Symbol_)
+  (x : Symbol_)
+  (N : Term_) :
+  x = y →
+  is_sub_v0 (var_ y) x N N
+
+-- if x ≠ y then y [ x := N ] = y
+| var_diff
+  (y : Symbol_)
+  (x : Symbol_)
+  (N : Term_) :
+  ¬ x = y →
+  is_sub_v0 (var_ y) x N (var_ y)
+
+-- (P Q) [ x := N ] = (P [ x := N ] Q [ x := N ])
+| app
+  (P : Term_)
+  (Q : Term_)
+  (x : Symbol_)
+  (N : Term_)
+  (P' : Term_)
+  (Q' : Term_) :
+  is_sub_v0 P x N P' →
+  is_sub_v0 Q x N Q' →
+  is_sub_v0 (app_ P Q) x N (app_ P' Q')
+
+-- if x = y then ( λ y . P ) [ x := N ] = ( λ y . P )
+| abs_same
+  (y : Symbol_)
+  (P : Term_)
+  (x : Symbol_)
+  (N : Term_) :
+  x = y →
+  is_sub_v0 (abs_ y P) x N (abs_ y P)
+
+| abs_diff_nel
+  (y : Symbol_)
+  (P : Term_)
+  (x : Symbol_)
+  (N : Term_) :
+  ¬ x = y →
+  x ∉ P.free_var_set →
+  is_sub_v0 (abs_ y P) x N (abs_ y P)
+
+| abs_diff
+  (y : Symbol_)
+  (P : Term_)
+  (x : Symbol_)
+  (N : Term_)
+  (P' : Term_) :
+  ¬ x = y →
+  y ∉ N.free_var_set →
+  is_sub_v0 P x N P' →
+  is_sub_v0 (abs_ y P) x N (abs_ y P')
+
+
+-------------------------------------------------------------------------------
+
+
 -- [1]
 
-
--- is_sub M x N L means M [ x := N ] = L
+/--
+  is_sub M x N L := True if and only if L is the result of replacing each free occurrence of x in M by N and no free occurrence of a variable in N becomes a bound occurrence in L.
+  M [ x := N ] = L
+-/
 inductive is_sub : Term_ → Symbol_ → Term_ → Term_ → Prop
 
 -- if x = y then y [ x := N ] = N
@@ -125,34 +190,3 @@ inductive is_sub_alt : Term_ → Symbol_ → Term_ → Term_ → Prop
 
 
 -------------------------------------------------------------------------------
-
-
-example
-  (y : Symbol_)
-  (P : Term_)
-  (x : Symbol_)
-  (N : Term_)
-  (P' : Term_)
-  (h1 : is_sub_alt P x N P')
-  (h2 : y ∉ N.free_var_set) :
-  is_sub_alt (abs_ y P) x N (abs_ y P') :=
-  by
-    apply is_sub_alt.abs
-    · exact h2
-    · rw [replace_free_self]
-      apply are_alpha_equiv_alt.refl
-    · rw [replace_free_self]
-      exact h1
-
-
-example
-  (y : Symbol_)
-  (P : Term_)
-  (x : Symbol_)
-  (N : Term_)
-  (P' : Term_)
-  (h1 : is_sub_alt P x N P')
-  (h2 : x ∉ P.free_var_set) :
-  is_sub_alt (abs_ y P) x N (abs_ y P') :=
-  by
-    sorry
